src/lemmas/inversion.lean
@@ -28,7 +28,7 @@ end
 theorem inversion_fn
   {Γ: cx typ} {x: var} {τ1 τ: typ} {e: exp}
   (et: has_typ Γ (exp.fn x τ1 e) τ)
-  : ∃ (τ2: typ), τ = typ.arrow τ1 τ2 ∧ has_typ (cx.insert x τ1 Γ) e τ2 :=
+  : ∃ (τ2: typ), τ = typ.arrow τ1 τ2 ∧ has_typ (cx.insert Γ x τ1) e τ2 :=
 begin
   cases et,
   existsi et_τ2,
